IronFleetDefault/ironfleet/src/Dafny/Distributed/Protocol/CausalMesh/message.dfy
@@ -1,11 +1,13 @@
 include "types.dfy"
+include "../../Common/Framework/Environment.s.dfy"
 
 module CausalMesh_Message_i {
     import opened CausalMesh_Types_i
+    import opened Environment_s
 
     datatype Message = 
-          Message_Invalid()
-        | Message_Read(key_read:Key, deps_read:Dependency)
+        //   Message_Invalid()
+          Message_Read(key_read:Key, deps_read:Dependency)
         | Message_Read_Reply(key_rreply:Key, vc_rreply:VectorClock, deps_rreply:Dependency)
         | Message_Write(key_write:Key, deps_write:Dependency, local:map<Key, Meta>)
         | Message_Write_Reply(key_wreply:Key, vc_wreply:VectorClock)
@@ -14,7 +16,7 @@ module CausalMesh_Message_i {
     predicate MessageValid(m:Message)
     {
         match m 
-            case Message_Invalid() => true
+            // case Message_Invalid() => true
             case Message_Read(key_read, deps_read) => key_read in Keys_domain && DependencyValid(deps_read)
             case Message_Read_Reply(key_rreply, vc_rreply, deps_rreply) => key_rreply in Keys_domain && VectorClockValid(vc_rreply) && DependencyValid(deps_rreply)
             case Message_Write(key_write, deps_write, local) => key_write in Keys_domain && DependencyValid(deps_write)
@@ -22,7 +24,10 @@ module CausalMesh_Message_i {
             case Message_Propagation(key, metas, start) => key in Keys_domain && forall m :: m in metas ==> MetaValid(m) && 0 <= start < Nodes
     }
 
-    datatype Packet = Packet(src:int, dst:int, msg:Message)
+    // datatype Packet = Packet(src:int, dst:int, msg:Message)
+    type Packet = LPacket<int, Message>
+    type CMEnvironment = LEnvironment<int, Message>
+    type CMIo = LIoOp<int, Message>
 
     predicate PacketValid(p:Packet)
     {
