IronFleetDefault/ironfleet/src/Dafny/Distributed/Protocol/CausalMesh/proof/action.dfy
@@ -1,0 +1,40 @@
+include "../distributed_system.dfy"
+include "../../../Common/Logic/Temporal/Rules.i.dfy"
+include "constants.dfy"
+
+module CausalMesh_Proof_Actions_i {
+import opened CausalMesh_Cache_i
+import opened CausalMesh_Message_i
+import opened CausalMesh_Types_i
+import opened Environment_s
+import opened CausalMesh_DistributedSystem_i
+import opened Temporal__Temporal_s
+import opened Collections__Maps2_s
+import opened CausalMesh_Proof_Constants_i
+import opened CausalMesh_proof_Assumptions_i
+
+  lemma lemma_ActionThatChangesServerIsThatServersAction(
+    b:Behavior<CMState>,
+    i:int,
+    idx:int
+  )
+    returns (ios:seq<CMIo>)
+    requires IsValidBehaviorPrefix(b, i+1)
+    requires 0 <= i
+    requires 0 <= idx < |b[i].servers|
+    requires 0 <= idx < |b[i+1].servers|
+    requires b[i+1].servers[idx] != b[i].servers[idx]
+    ensures  b[i].environment.nextStep.LEnvStepHostIos?
+    ensures  0 <= idx < Nodes
+    ensures  b[i].environment.nextStep.actor == idx
+    ensures  ios == b[i].environment.nextStep.ios
+    ensures  CMNext(b[i], b[i+1])
+    ensures  CMNextServer(b[i], b[i+1], idx, ios)
+  {
+    lemma_AssumptionsMakeValidTransition(b, i);
+    lemma_ConstantsAllConsistent(b, i);
+    assert CMNext(b[i], b[i+1]);
+    ios :| CMNextServer(b[i], b[i+1], idx, ios);
+  }
+
+}
