IronFleetDefault/ironfleet/src/Dafny/Distributed/Protocol/CausalMesh/proof/assumptions.dfy
@@ -1,0 +1,23 @@
+include "../distributed_system.dfy"
+include "../../../Common/Collections/Maps2.i.dfy"
+
+module CausalMesh_proof_Assumptions_i {
+import opened CausalMesh_Cache_i
+import opened CausalMesh_Message_i
+import opened CausalMesh_Types_i
+import opened Environment_s
+import opened CausalMesh_DistributedSystem_i
+import opened Temporal__Temporal_s
+import opened Collections__Maps2_s
+
+predicate IsValidBehaviorPrefix(
+  b:Behavior<CMState>,
+  i:int
+  )
+{
+  && imaptotal(b)
+  && CMInit(b[0])
+  && (forall j {:trigger CMNext(b[j], b[j+1])} :: 0 <= j < i ==> CMNext(b[j], b[j+1]))
+}
+
+}
