IronFleetDefault/ironfleet/src/Dafny/Distributed/Protocol/CausalMesh/proof/causalcut.dfy
@@ -1,0 +1,161 @@
+include "../distributed_system.dfy"
+include "action.dfy"
+include "../../../Common/Collections/Seqs.s.dfy"
+
+module CausalMesh_Proof_CausalCut_i {
+import opened CausalMesh_Cache_i
+import opened CausalMesh_Message_i
+import opened CausalMesh_Types_i
+import opened Environment_s
+import opened CausalMesh_DistributedSystem_i
+import opened CausalMesh_Proof_Actions_i
+import opened Temporal__Temporal_s
+import opened CausalMesh_proof_Assumptions_i
+import opened CausalMesh_Proof_Constants_i
+import opened Collections__Seqs_s
+// import opened Collections__Sets_i
+import opened Collections__Maps2_s
+
+function {:opaque} ConvertBehaviorSeqToImap<T>(s:seq<T>):imap<int, T>
+  requires |s| > 0
+  ensures  imaptotal(ConvertBehaviorSeqToImap(s))
+  ensures  forall i :: 0 <= i < |s| ==> ConvertBehaviorSeqToImap(s)[i] == s[i]
+{
+  imap i {:trigger s[i]} :: if i < 0 then s[0] else if 0 <= i < |s| then s[i] else last(s)
+}
+
+lemma lemma_AllServersAreCausalSet(
+    low_level_behavior:seq<CMState>
+)
+    requires |low_level_behavior| > 0 
+    requires CMInit(low_level_behavior[0])
+    requires forall i {:trigger CMNext(low_level_behavior[i], low_level_behavior[i+1])} :: 
+                0 <= i < |low_level_behavior| - 1 ==> CMNext(low_level_behavior[i], low_level_behavior[i+1])
+    ensures forall i :: 0 <= i < |low_level_behavior| ==> AllServersAreCausalCut(low_level_behavior[i])
+{
+    assert AllServersAreCausalCut(low_level_behavior[0]);
+
+    var b := ConvertBehaviorSeqToImap(low_level_behavior);
+    lemma_AllServersAreCausalSetPrefix(b, |low_level_behavior|-1);
+}
+
+lemma lemma_AllServersAreCausalSetPrefix(
+    b:Behavior<CMState>,
+    i:int
+)
+    requires 0 <= i 
+    requires IsValidBehaviorPrefix(b, i)
+    requires AllServersAreCausalCut(b[0])
+    ensures forall j :: 0 <= j <= i ==> AllServersAreCausalCut(b[j])
+{
+    if i == 0 {
+        return;
+    }
+
+    lemma_ConstantsAllConsistent(b, i-1);
+    lemma_ConstantsAllConsistent(b, i);
+
+    lemma_AllServersAreCausalSetPrefix(b, i-1);
+    assert forall j :: 0 <= j < i ==> AllServersAreCausalCut(b[j]);
+
+    lemma_CMNextRemainsCausalCut(b, i-1);
+    assert AllServersAreCausalCut(b[i]);
+}
+
+// lemma lemma_CMNextRemainsCausalCut(low_level_behavior:seq<CMState>, i:int)
+//     requires |low_level_behavior| > 1
+//     requires 0 <= i < |low_level_behavior| - 1
+//     requires CMNext(low_level_behavior[i], low_level_behavior[i+1])
+//     requires AllServersAreCausalCut(low_level_behavior[i])
+//     // ensures AllServersAreCausalCut(low_level_behavior[i+1])
+// {
+//     var ps := low_level_behavior[i];
+//     var ps' := low_level_behavior[i+1];
+
+//     if ps.servers == ps'.servers {
+//         assert AllServersAreCausalCut(ps');
+//     } 
+//     // else {
+//     //     assume AllServersAreCausalCut(ps');
+//     // }
+// }
+
+lemma lemma_CMNextRemainsCausalCut(b:Behavior<CMState>, i:int)
+    requires IsValidBehaviorPrefix(b, i+1)
+    requires 0 <= i
+    // requires 0 <= i < |low_level_behavior| - 1
+    requires CMNext(b[i], b[i+1])
+    requires AllServersAreCausalCut(b[i])
+    ensures AllServersAreCausalCut(b[i+1])
+{
+    var ps := b[i];
+    var ps' := b[i+1];
+
+    if ps.servers == ps'.servers {
+        assert AllServersAreCausalCut(ps');
+    } 
+    else {
+        var idx :| 0 <= idx < |ps.servers| && ps.servers[idx] != ps'.servers[idx];
+        lemma_CMNextServerRemainsCausalCut(b, i, idx);
+    }
+}
+
+lemma lemma_CMNextServerRemainsCausalCut(b:Behavior<CMState>, i:int, idx:int)
+    requires IsValidBehaviorPrefix(b, i+1)
+    requires 0 <= i
+    requires 0 <= idx < |b[i].servers|
+    requires 0 <= idx < |b[i+1].servers|
+    requires b[i].servers[idx] != b[i+1].servers[idx]
+    requires AllServersAreCausalCut(b[i])
+    ensures AllServersAreCausalCut(b[i+1])
+{
+    var s := b[i].servers[idx].s;
+    var s' := b[i+1].servers[idx].s;
+
+    var ios := lemma_ActionThatChangesServerIsThatServersAction(b, i, idx);
+    assert CMNextServer(b[i], b[i+1], idx, ios);
+    assert LServerNext(b[i].servers[idx], b[i+1].servers[idx], ios);
+    assert ServerValid(s);
+
+    assert ios[0].LIoOpReceive?;
+    var p := ios[0].r;
+    var sp := ExtractSentPacketsFromIos(ios);
+    assert p.msg.Message_Read? || p.msg.Message_Write? || p.msg.Message_Propagation?;
+
+    assert ServerProcessPacket(s, s', ios);
+
+    if p.msg.Message_Read? {
+        assert ReceiveRead(s, s', p, sp);
+        lemma_PullDeps2RemainsCausalCut(s.icache, s.ccache, p.msg.deps_read);
+        assert CausalCut(s'.ccache);
+    } 
+    else 
+    if p.msg.Message_Write? {
+        assert ReceiveWrite(s, s', p, sp);
+        assert CausalCut(s'.ccache);
+    } 
+    else {
+        assert p.msg.Message_Propagation?;
+        assert ReceivePropagate(s, s', p, sp);
+        if s.next == p.msg.start {
+            var deps := set x | x in p.msg.metas :: x.deps;
+            var new_deps := FoldDependency(map[], deps);
+            lemma_PullDeps2RemainsCausalCut(s.icache, s.ccache, new_deps);
+        }
+        
+        assert CausalCut(s'.ccache);
+    }
+ 
+}
+
+lemma {:axiom} lemma_PullDeps2RemainsCausalCut(icache:ICache, ccache:CCache, deps:Dependency)
+    requires ICacheValid(icache)
+    requires CCacheValid(ccache)
+    requires forall k :: k in ccache ==> k in icache
+    requires DependencyValid(deps)
+    requires forall k :: k in deps ==> k in icache
+    requires CausalCut(ccache)
+    ensures var (new_icache, new_ccache) := PullDeps2(icache, ccache, deps);
+            CausalCut(new_ccache)
+
+}
