IronFleetDefault/ironfleet/src/Dafny/Distributed/Protocol/CausalMesh/proof/constants.dfy
@@ -1,0 +1,53 @@
+include "../distributed_system.dfy"
+include "../../../Common/Logic/Temporal/Rules.i.dfy"
+include "assumptions.dfy"
+
+module CausalMesh_Proof_Constants_i {
+import opened CausalMesh_Cache_i
+import opened CausalMesh_Message_i
+import opened CausalMesh_Types_i
+import opened Environment_s
+import opened CausalMesh_DistributedSystem_i
+import opened Temporal__Temporal_s
+import opened Temporal__Rules_i
+import opened Temporal__Heuristics_i
+import opened CausalMesh_proof_Assumptions_i
+
+
+predicate ConstantsAllConsistentInv(ps:CMState)
+{
+    && |ps.servers| == Nodes
+    && |ps.clients| == Clients
+    && (forall idx :: 0 <= idx < Nodes ==> ps.servers[idx].s.id == idx)
+    && (forall idx :: 0 <= idx < Clients ==> ps.clients[idx].c.id == idx + Nodes)
+}
+
+lemma lemma_AssumptionsMakeValidTransition(
+  b:Behavior<CMState>,
+  i:int
+  )
+  requires IsValidBehaviorPrefix(b, i+1)
+  requires 0 <= i
+  ensures  CMNext(b[i], b[i+1])
+{
+}
+
+
+lemma lemma_ConstantsAllConsistent(
+  b:Behavior<CMState>,
+  i:int
+  )
+  requires IsValidBehaviorPrefix(b, i)
+  requires 0 <= i
+  ensures  ConstantsAllConsistentInv(b[i])
+{
+  TemporalAssist();
+
+  if i > 0
+  {
+    lemma_ConstantsAllConsistent(b, i-1);
+    lemma_AssumptionsMakeValidTransition(b, i-1);
+  }
+}
+
+}
